integration/talos/FirTalos/ConcreteRuntimeExamples.lean
@@ -136,7 +136,7 @@ private def compilerShapedScalarMutationProgram : Fir.LeanIR.ImpureProgram :=
       .let (letDecl y LCNF.ImpureType.tobject (.lit (.nat 2))) <|
       .let (letDecl p objType (.ctor layoutInfo #[.fvar x])) <|
       .let (letDecl u usizeType (.lit (.usize 55))) <|
-      .uset p 0 u <|
+      .uset p 1 u <|
       .let (letDecl s u64Type (.lit (.uint64 66))) <|
       .sset p 2 0 s u64Type <|
       .oset p 0 (.fvar y) <|
